Exercise 2.2

\begin{align*}
Q_{n+1} &= Q_n + \alpha_n[R_n-Q_n] \\
&= \alpha_nR_n + (1-\alpha_n)Q_n \\
&= \alpha_nR_n + (1-\alpha_n)[\alpha_{n-1}R_{n-1} + (1-\alpha_{n-1})Q_{n-1}] \\
&= \alpha_nR_n + (1-\alpha_n)\alpha_{n-1}R_{n-1} + (1-\alpha_n)(1-\alpha_{n-1})Q_{n-1} \\
&= \alpha_nR_n + (1-\alpha_n)\alpha_{n-1}R_{n-1} + \cdots + \prod_{i=2}^{n}(1-\alpha_i)\alpha_1R_1 + \prod_{i=1}^{n}(1-\alpha_i)Q_1 \\
&= \alpha_nR_n + \sum_{i=1}^{n-1}\prod_{j=i+1}^{n}(1-\alpha_j)\alpha_iR_i + \prod_{i=1}^{n}(1-\alpha_i)Q_1
\end{align*}

